go.sh
@@ -1,2 +1,3 @@
 #/var/tmp/coq-8.2pl2/bin/coqide -I lib $1 $2 $3 $4 &
+# source local_settings.sh
 coqide -I lib/v3 $1 $2 $3 $4 &
